Need to show logrel satisfies renaming/weakening

syntax.sig
@@ -3,10 +3,8 @@ ty : Type
 
 Lam : ty -> (tm -> tm) -> tm
 App : tm -> tm -> tm
-TmK : tm
 TmUnit : tm
 
 
 Fun : ty -> ty -> ty
-TyK : ty
 TyUnit : ty
